cfrontend/ChkCgenproof.v
@@ -24,3 +24,25 @@ Require Import ChkCgen ChkCgenspec.
 Definition match_prog (p: ChkCsyntax.program) (tp: Csyntax.program) :=
   match_program (fun ctx f tf => tr_fundef f tf) eq p tp
   /\ prog_types tp = prog_types p.
+
+Lemma transf_program_match:
+  forall p tp, transl_program p = OK tp -> match_prog p tp.
+Proof.
+  unfold transl_program; intros. monadInv H. split; auto.
+  unfold program_of_program; simpl. destruct x; simpl.
+  eapply match_transform_partial_program_contextual. eexact EQ.
+  intros. apply transl_fundef_spec; auto.
+Qed.
+
+Instance TransfChkCGenLink : TransfLink match_prog.
+Proof.
+  red; intros. eapply Ctypes.link_match_program; eauto.
+  - intros.
+    Local Transparent Linker_fundef.
+    simpl in *; unfold link_fundef in *. inv H3; inv H4; try discriminate.
+    destruct ef; inv H2. exists (Internal tf); split; auto. constructor; auto.
+    destruct ef; inv H2. exists (Internal tf); split; auto. constructor; auto.
+    destruct (external_function_eq ef ef0 && typelist_eq targs targs0 &&
+                                   type_eq tres tres0 && calling_convention_eq cconv cconv0); inv H2.
+    exists (External ef targs tres cconv); split; auto. constructor.
+Qed.
